src/ipm_tactics.v
@@ -1,0 +1,15 @@
+From iris.proofmode Require Import tactics.
+From iris_named_props Require Import named_props.
+
+Ltac iPureGoal :=
+  rewrite bi.pure_True;
+  first (rewrite (left_id (True)%I) || rewrite (right_id (True)%I));
+  last first.
+
+Lemma pure_named_True {PROP} name (φ : Prop) : φ → (name ∷ ⌜φ⌝) ⊣⊢@{PROP} True.
+Proof. apply bi.pure_True. Qed.
+
+Ltac iPureGoalNamed name :=
+  rewrite (pure_named_True name);
+  first (rewrite (left_id (True)%I) || rewrite (right_id (True)%I));
+  last first.
